Term_system.v
@@ -1,0 +1,253 @@
+(* Copland specific event systems *)
+
+(* LICENSE NOTICE
+
+Copyright (c) 2018 The MITRE Corporation.
+All Rights Reserved.
+
+This proof script is free software: you can redistribute it and/or
+modify it under the terms of the BSD License as published by the
+University of California.  See license.txt for details. *)
+
+(** Copland specific event systems. *)
+
+Require Import Omega Preamble More_lists Term Event_system.
+
+(** Construct an event system from an annotated term, place, and
+    evidence. *)
+
+Fixpoint ev_sys (t: AnnoTerm) : EvSys Ev :=
+  match t with
+  | aasp (i, j) x => leaf (i, j) (asp_event i x)
+  | aatt (i, j) q x =>
+    before (i, j)
+      (leaf (i, S i) (req i q (unanno x)))
+      (before (S i, j)
+              (ev_sys x)
+              (leaf (pred j, j) (rpy (pred j) q)))
+  | alseq r x y => before r (ev_sys x)
+                          (ev_sys y)
+  | abseq (i, j) s x y =>
+    before (i, j)
+           (leaf (i, S i)
+                 (split i ))
+           (before (S i, j)
+                   (before (S i, (pred j))
+                           (ev_sys x)
+                           (ev_sys y))
+                   (leaf ((pred j), j)
+                   (join (pred j) )))
+  | abpar (i, j) s x y =>
+    before (i, j)
+           (leaf (i, S i)
+                 (split i ))
+           (before (S i, j)
+                   (merge (S i, (pred j))
+                          (ev_sys x)
+                          (ev_sys y))
+                   (leaf ((pred j), j)
+                   (join (pred j) )))
+  end.
+
+Lemma evsys_range:
+  forall t,
+    es_range (ev_sys t) = range t.
+Proof.
+  induction t; intros; simpl; auto;
+    repeat expand_let_pairs; simpl; auto.
+Qed.
+
+Lemma well_structured_evsys:
+  forall t,
+    well_formed t ->
+    well_structured ev (ev_sys t).
+Proof.
+  induction t; intros; inv H; simpl;
+    repeat expand_let_pairs; destruct r as [i k];
+      simpl in *; subst; auto.
+  - apply ws_leaf_event; auto;
+      destruct a; simpl; auto.
+  - apply ws_before; simpl; auto.
+    rewrite H4.
+    apply ws_before; simpl; auto; rewrite evsys_range; auto.
+  - apply ws_before; auto; repeat rewrite evsys_range; auto.
+  - repeat (apply ws_before; simpl in *; auto; repeat rewrite evsys_range; auto).
+  - repeat (apply ws_before; simpl in *; auto; repeat rewrite evsys_range; auto).
+    repeat (apply ws_merge; simpl in *; auto; repeat rewrite evsys_range; auto).
+Qed.
+
+(** The events in the event system correspond to the events associated
+    with a term, a place, and some evidence. *)
+
+Lemma evsys_events:
+  forall t ev,
+    well_formed t ->
+    ev_in ev (ev_sys t) <-> events t ev.
+Proof.
+  split; induction t; intros; inv H; simpl in *;
+    repeat expand_let_pairs; simpl in *.
+  - inv H0; auto; destruct a; simpl; auto.
+  - inv H0; auto.
+    inv H2; auto.
+    inv H2; auto.
+    inv H1; auto.
+
+    apply evtsattrpy. simpl. omega.
+    
+
+
+(*
+    rewrite H6 in H0; clear H6; simpl in H0.
+    rewrite H5 in H0; clear H5; simpl in H0.
+    inv H0. inv H2.
+    inv H4; auto.
+    econstructor. 
+
+
+    auto. inv H2; auto.
+    inv H1; auto. *)
+  - inv H0; auto.
+  - rewrite H9 in H0; simpl in H0.
+    inv H0; inv H2; auto; inv H1; auto.
+  - rewrite H9 in H0; simpl in H0.
+    inv H0; inv H2; auto; inv H1; auto.
+  - inv H0; auto.
+  - inv H0; auto.
+
+
+
+
+    rewrite H6; simpl.
+    
+    Print ev_in.
+    apply ein_beforer.
+    apply ein_beforer.
+    assert (snd (range t) = i). omega.
+    subst.
+    apply ein_leaf.
+
+  - inv H0; auto.
+  - inv H0; auto.
+    apply ein_beforer.
+    apply ein_beforer.
+    assert ((Init.Nat.pred (snd r) = i)). omega. subst.
+    apply ein_leaf.
+
+ -   inv H0; auto.
+    apply ein_beforer.
+    apply ein_beforer.
+    assert ((Init.Nat.pred (snd r) = i)). omega. subst.
+    apply ein_leaf.
+Qed.
+
+(** Maximal events are unique. *)
+
+Lemma supreme_unique:
+  forall t,
+    well_formed t ->
+    exists ! v, supreme (ev_sys t) v.
+Proof.
+  intros.
+  assert (G: well_structured ev (ev_sys t)).
+  apply well_structured_evsys; auto.
+  rewrite <- unique_existence.
+  split.
+  - exists (max (ev_sys t)).
+    apply supreme_max with (ev:=ev); auto.
+  - unfold uniqueness.
+    intros.
+    rewrite <- sup_supreme with (ev:=ev) in H0; auto.
+    rewrite <- sup_supreme with (ev:=ev) in H1; auto.
+    revert H1.
+    revert H0.
+    revert G.
+    induction H; intros.
+    + destruct r as [i j]; simpl in *.
+      inv H0; inv H1; auto.
+    + destruct r as [i j]; simpl in *.
+      repeat apply before_sup in H2.
+      repeat apply before_sup in H3.
+      inv H2; inv H3; auto.
+    + destruct r as [i j]; simpl in *.
+      repeat apply before_sup in H4.
+      repeat apply before_sup in H5.
+      eapply IHwell_formed2 in H4; eauto.
+      inv G; auto.
+    + destruct r as [i j]; simpl in *.
+      repeat apply before_sup in H4.
+      repeat apply before_sup in H5.
+      inv H4; inv H5; auto.
+    + destruct r as [i j]; simpl in *.
+      repeat apply before_sup in H4.
+      repeat apply before_sup in H5.
+      inv H4; inv H5; auto.
+Qed.
+
+Lemma evsys_max_unique:
+  forall t,
+    well_formed t ->
+    unique (supreme (ev_sys t)) (max (ev_sys t)).
+Proof.
+  intros.
+  assert (G: well_structured ev (ev_sys t)).
+  apply well_structured_evsys; auto.
+  unfold unique.
+  split.
+  apply supreme_max with (ev:=ev); auto.
+  intros.
+  rewrite <- sup_supreme with (ev:=ev) in H0; auto.
+  revert H0.
+  revert G.
+  revert x'.
+  induction H; intros; destruct r as [i j]; inv G; simpl in *; auto.
+  - inv H0; auto.
+  - repeat apply before_sup in H2.
+    inv H2; auto.
+  - repeat apply before_sup in H4.
+    apply IHwell_formed2 in H4; auto.
+  - repeat apply before_sup in H4.
+    inv H4; auto.
+  - repeat apply before_sup in H4.
+    inv H4; auto.
+Qed.
+
+(** Maximal event evidence output matches [aeval]. *)
+
+(*
+Definition out_ev v :=
+  match v with
+  | copy _ _ e => e
+  | kmeas _ _ _ _ _ e => e
+  | umeas _ _ _ _ e => e
+  | sign _ _ e => e
+  | hash _ _ e => e
+  | req _ _ _ t => mt
+  | rpy _ _ _ e => e
+  | split _ _ _ _ e => e
+  | join _ _ _ _ e => e
+  end.
+
+Lemma max_eval:
+  forall t p e,
+    well_formed t ->
+    out_ev (max (ev_sys t p e)) = aeval t p e.
+Proof.
+  intros.
+  revert e.
+  revert p.
+  induction H; intros; simpl; repeat expand_let_pairs; simpl; auto.
+  destruct x; simpl; auto.
+Qed. *)
+
+(** lseq is associative relative to the event semantics *)
+
+Lemma lseq_assoc:
+  forall t1 t2 t3 i,
+    same_rel
+      (ev_sys (snd (anno (lseq t1 (lseq t2 t3)) i)))
+      (ev_sys (snd (anno (lseq (lseq t1 t2) t3) i))).
+Proof.
+  intros; simpl.
+  repeat expand_let_pairs; simpl.
+  apply before_associative_pairs.
+Qed.
