Trace.v
@@ -1,0 +1,674 @@
+(* Traces and their relation to event systems *)
+
+(* LICENSE NOTICE
+
+Copyright (c) 2018 The MITRE Corporation.
+All Rights Reserved.
+
+This proof script is free software: you can redistribute it and/or
+modify it under the terms of the BSD License as published by the
+University of California.  See license.txt for details. *)
+
+(** Traces and their relation to event systems. *)
+
+Require Import List.
+Import List.ListNotations.
+Open Scope list_scope.
+Require Import Omega Preamble More_lists Term Event_system Term_system.
+
+(** * Shuffles
+
+    A trace is a list of events.  [shuffle] merges two traces as is
+    done by parallel execution.  The order of events in the traces to
+    be merged does not change, but all other interleavings are
+    allowed.  *)
+
+Inductive shuffle: list Ev -> list Ev -> list Ev -> Prop :=
+| shuffle_nil_left: forall es, shuffle [] es es
+| shuffle_nil_right: forall es, shuffle es [] es
+| shuffle_left:
+    forall e es0 es1 es2,
+      shuffle es0 es1 es2 ->
+      shuffle (e :: es0) es1 (e :: es2)
+| shuffle_right:
+    forall e es0 es1 es2,
+      shuffle es0 es1 es2 ->
+      shuffle es0 (e :: es1) (e :: es2).
+Hint Constructors shuffle.
+
+Lemma shuffle_length:
+  forall es0 es1 es2,
+    shuffle es0 es1 es2 ->
+    length es0 + length es1 = length es2.
+Proof.
+  intros.
+  induction H; simpl; auto; omega.
+Qed.
+
+Lemma shuffle_in_left:
+  forall e es0 es1 es2,
+    shuffle es0 es1 es2 ->
+    In e es0 ->
+    In e es2.
+Proof.
+  intros.
+  induction H; auto.
+  - inv H0; tauto.
+  - destruct H0.
+    + subst; simpl; auto.
+    + simpl; auto.
+  - apply IHshuffle in H0.
+    simpl; auto.
+Qed.
+
+Lemma shuffle_in_right:
+  forall e es0 es1 es2,
+    shuffle es0 es1 es2 ->
+    In e es1 ->
+    In e es2.
+Proof.
+  intros.
+  induction H; auto.
+  - inv H0; tauto.
+  - apply IHshuffle in H0.
+    simpl; auto.
+  - destruct H0.
+    subst; simpl; auto.
+    apply IHshuffle in H0.
+    simpl; auto.
+Qed.
+
+Lemma shuffle_in:
+  forall e es0 es1 es2,
+    shuffle es0 es1 es2 ->
+    In e es2 <-> In e es0 \/ In e es1.
+Proof.
+  split; intros.
+  - induction H; simpl; auto;
+    simpl in H0; destruct H0; auto;
+      apply IHshuffle in H0; tauto.
+  - destruct H0; auto.
+    + eapply shuffle_in_left in H; eauto.
+    + eapply shuffle_in_right in H; eauto.
+Qed.
+
+Lemma shuffle_in_skipn_left:
+  forall i e es0 es1 es2,
+    shuffle es0 es1 es2 ->
+    In e (skipn i es0) ->
+    In e (skipn i es2).
+Proof.
+  intros.
+  revert H0.
+  revert e.
+  revert i.
+  induction H; intros; auto.
+  - rewrite skipn_nil in H0.
+    inv H0.
+  - destruct i.
+    + simpl in *; auto; destruct H0; auto.
+      specialize IHshuffle with (i:=0).
+      simpl in IHshuffle; auto.
+    + simpl in *; auto.
+  - apply IHshuffle in H0.
+    apply in_skipn_cons; auto.
+Qed.
+
+Lemma shuffle_in_skipn_right:
+  forall i e es0 es1 es2,
+    shuffle es0 es1 es2 ->
+    In e (skipn i es1) ->
+    In e (skipn i es2).
+Proof.
+  intros.
+  revert H0.
+  revert e.
+  revert i.
+  induction H; intros; auto.
+  - rewrite skipn_nil in H0.
+    inv H0.
+  - apply IHshuffle in H0.
+    apply in_skipn_cons; auto.
+  - destruct i; simpl in *; auto.
+    destruct H0; auto; right.
+    specialize IHshuffle with (i:=0).
+    simpl in *; auto.
+Qed.
+
+Lemma shuffle_earlier_left:
+  forall es0 es1 es2 e0 e1,
+    earlier es0 e0 e1 ->
+    shuffle es0 es1 es2 ->
+    earlier es2 e0 e1.
+Proof.
+  intros.
+  destruct H as [i H].
+  destruct H.
+  unfold earlier.
+  revert H.
+  revert H1.
+  revert i.
+  induction H0; intros.
+  - rewrite firstn_nil in H; inv H.
+  - exists i; auto.
+  - destruct i.
+    + simpl in *; tauto.
+    + simpl in H, H1.
+      destruct H; subst.
+      * exists (S i); simpl; auto.
+        split; auto.
+        eapply shuffle_in_skipn_left; eauto.
+      * eapply IHshuffle in H1; eauto.
+        destruct H1 as [n].
+        destruct H1.
+        exists (S n); simpl; auto.
+  - eapply IHshuffle in H1; eauto.
+    destruct H1 as [n].
+    destruct H1.
+    exists (S n); simpl; auto.
+Qed.
+
+Lemma shuffle_earlier_right:
+  forall es0 es1 es2 e0 e1,
+    earlier es1 e0 e1 ->
+    shuffle es0 es1 es2 ->
+    earlier es2 e0 e1.
+Proof.
+  intros.
+  destruct H as [i H].
+  destruct H.
+  unfold earlier.
+  revert H.
+  revert H1.
+  revert i.
+  induction H0; intros.
+  - exists i; auto.
+  - rewrite firstn_nil in H; inv H.
+  - eapply IHshuffle in H1; eauto.
+    destruct H1 as [n].
+    destruct H1.
+    exists (S n); simpl; auto.
+  - destruct i.
+    + simpl in *; tauto.
+    + simpl in H, H1.
+      destruct H; subst.
+      * exists (S i); simpl; auto.
+        split; auto.
+        eapply shuffle_in_skipn_right; eauto.
+      * eapply IHshuffle in H1; eauto.
+        destruct H1 as [n].
+        destruct H1.
+        exists (S n); simpl; auto.
+Qed.
+
+Lemma shuffle_nodup_append:
+  forall tr0 tr1 tr2,
+    NoDup tr0 -> NoDup tr1 ->
+    disjoint_lists tr0 tr1 ->
+    shuffle tr0 tr1 tr2 ->
+    NoDup tr2.
+Proof.
+  intros.
+  induction H2; auto.
+  - apply NoDup_cons.
+    + intro.
+      eapply shuffle_in in H2.
+      apply H2 in H3.
+      destruct H3.
+      * inv H; tauto.
+      * apply H1 in H3; simpl; auto.
+    + apply IHshuffle; auto.
+      * inv H; auto.
+      * unfold disjoint_lists; intros.
+        apply H1 in H4; auto.
+        simpl; auto.
+  - apply NoDup_cons.
+    + intro.
+      eapply shuffle_in in H2.
+      apply H2 in H3.
+      destruct H3.
+      * apply H1 in H3; simpl in H3; auto.
+      * inv H0; tauto.
+    + apply IHshuffle; auto.
+      * inv H0; auto.
+      * unfold disjoint_lists; intros.
+        apply H1 in H3; auto.
+        simpl in H3; auto.
+Qed.
+
+(** * Big-Step Semantics
+
+    The traces associated with an annotated term are defined
+    inductively. *)
+
+Inductive trace: AnnoTerm ->
+                 list Ev -> Prop :=
+| tasp: forall r x,
+    trace (aasp r x) [(asp_event (fst r) x)]
+| tatt: forall r x q tr1,
+    trace x tr1 ->
+    trace (aatt r q x)
+          ((req (fst r) q (unanno x))
+             :: tr1 ++
+             [(rpy (pred (snd r)) q)])
+| tlseq: forall r x y tr0 tr1,
+    trace x tr0 ->
+    trace y tr1 ->
+    trace (alseq r x y) (tr0 ++ tr1)
+| tbseq: forall r s x y tr0 tr1,
+    trace x tr0 ->
+    trace y tr1 ->
+    trace (abseq r s x y)
+          ((split (fst r))
+             :: tr0 ++ tr1 ++
+             [(join (pred (snd r)) )])
+| tbpar: forall r s x y tr0 tr1 tr2,
+    trace x tr0 ->
+    trace y tr1 ->
+    shuffle tr0 tr1 tr2 ->
+    trace (abpar r s x y)
+          ((split (fst r) )
+             :: tr2 ++
+             [(join (pred (snd r)))]).
+Hint Resolve tasp.
+
+Lemma trace_length:
+  forall t tr,
+    trace t tr -> esize t = length tr.
+Proof.
+  induction t; intros; inv H;
+    simpl; auto; rewrite app_length; simpl; auto.
+  - apply IHt in H4; omega.
+  - apply IHt1 in H5.
+    apply IHt2 in H6.
+    rewrite app_length. simpl in *. omega.
+  - apply IHt1 in H5.
+    apply IHt2 in H6.
+    apply shuffle_length in H7. omega.
+Qed.
+
+(** The events in a trace correspond to the events associated with an
+    annotated term, a place, and some evidence. *)
+
+Lemma trace_events:
+  forall t tr v,
+    well_formed t ->
+    trace t tr ->
+    In v tr <-> events t v.
+Proof.
+  split; intros.
+  - induction H0; inv H.
+    + inv H1; try inv H.
+      destruct x; constructor; auto.
+    + inv H1.
+      constructor; auto.
+      rewrite in_app_iff in H.
+      destruct H.
+      apply evtsatt; auto.
+      inv H; try inv H1.
+      rewrite H7; simpl.
+      apply evtsattrpy; auto.
+    + rewrite in_app_iff in H1.
+      destruct H1.
+      * apply evtslseql; auto.
+      * apply evtslseqr; auto.
+    + destruct H1; subst.
+      apply evtsbseqsplit; auto.
+      apply in_app_iff in H; destruct H.
+      apply evtsbseql; auto.
+      apply in_app_iff in H; destruct H.
+      apply evtsbseqr; auto.
+      destruct H; subst.
+      rewrite H9.
+      apply evtsbseqjoin; auto.
+      inv H.
+    + destruct H1; subst.
+      apply evtsbparsplit; auto.
+      apply in_app_iff in H; destruct H.
+      apply shuffle_in with (e:=v) in H0.
+      apply H0 in H.
+      destruct H.
+      apply evtsbparl; auto.
+      apply evtsbparr; auto.
+      rewrite H10 in H; simpl in H.
+      destruct H; try tauto; subst.
+      apply evtsbparjoin; auto.
+  - induction H0; inv H.
+    + inv H1; destruct r as [i j]; simpl in *; auto.
+    + simpl; rewrite in_app_iff; simpl.
+      inv H1; auto.
+      right; right.
+      rewrite H8; simpl; auto.
+    + rewrite in_app_iff.
+      inv H1; auto.
+    + simpl.
+      rewrite in_app_iff.
+      rewrite in_app_iff.
+      simpl.
+      inv H1; auto.
+      rewrite H10 in *.
+      auto.
+    + simpl.
+      rewrite in_app_iff.
+      simpl.
+      inv H1; auto.
+      * apply IHtrace1 in H11; auto.
+        eapply shuffle_in_left in H0; eauto.
+      * apply IHtrace2 in H11; auto.
+        eapply shuffle_in_right in H0; eauto.
+      * rewrite H11 in *; auto.
+Qed.
+
+Lemma trace_range:
+  forall t tr v,
+    well_formed t ->
+    trace t tr ->
+    In v tr ->
+    fst (range t) <= ev v < snd (range t).
+Proof.
+  intros.
+  rewrite trace_events in H1; eauto.
+  eapply events_range; eauto.
+Qed.
+
+Lemma trace_range_event:
+  forall t tr i,
+    well_formed t ->
+    trace t tr ->
+    fst (range t) <= i < snd (range t) ->
+    exists v, In v tr /\ ev v = i.
+Proof.
+  intros.
+  eapply events_range_event in H1; eauto.
+  destruct H1 as [v G]; destruct G as [G]; subst.
+  rewrite <- trace_events in G; eauto.
+Qed.
+
+Lemma trace_injective_events:
+  forall t tr v0 v1,
+    well_formed t ->
+    trace t tr ->
+    In v0 tr -> In v1 tr ->
+    ev v0 = ev v1 ->
+    v0 = v1.
+Proof.
+  intros.
+  rewrite trace_events in H1; eauto.
+  rewrite trace_events in H2; eauto.
+  eapply events_injective; eauto.
+Qed.
+
+Lemma nodup_trace:
+  forall t tr,
+    well_formed t ->
+    trace t tr ->
+    NoDup tr.
+Proof.
+  induction t; intros; inv H; inv H0.
+  - constructor; auto; constructor.
+  - destruct r as [i j]; simpl in *; subst; simpl.
+    apply NoDup_cons.
+    + intro.
+      apply in_app_iff in H.
+      destruct H.
+      * eapply trace_range in H7; eauto.
+        simpl in *.
+        omega.
+      * inv H.
+        discriminate H0.
+        inv H0.
+    + apply nodup_append; unfold disjoint_lists; auto; intros.
+     (* * eapply IHt; eauto.*)
+      * constructor; auto; constructor.
+      * inv H0.
+        eapply trace_range in H7; eauto.
+        simpl in *.
+        omega.
+        inv H1.
+ (* - apply nodup_append; unfold disjoint_lists; auto; intros.
+    eapply IHt1; eauto.
+    eapply IHt2; eauto.
+    eapply trace_range in H11; eauto.
+    eapply trace_range in H12; eauto.
+    omega. *)
+  - apply nodup_append; unfold disjoint_lists; auto; intros.
+    + eapply trace_range in H10; eauto.
+      eapply trace_range in H9; eauto.
+        simpl in *.
+        omega.
+    
+  - destruct r as [i j]; simpl in *; subst; simpl.
+    apply NoDup_cons.
+    + intro.
+      repeat rewrite in_app_iff in H.
+      repeat destruct_disjunct.
+      * eapply trace_range in H10; eauto.
+        simpl in H10.
+        omega.
+      * eapply trace_range in H11; eauto.
+        simpl in H11.
+        apply well_formed_range in H5; auto.
+        omega.
+      * inv H.
+        discriminate H0.
+        inv H0.
+    + apply nodup_append; unfold disjoint_lists; auto; intros.
+     (* * eapply IHt1; eauto.*)
+      * 
+
+        apply nodup_append; unfold disjoint_lists; auto; intros.
+       (* -- eapply IHt2; eauto. *)
+        -- apply NoDup_cons.
+           intro; inv H.
+           constructor.
+        -- inv H0.
+           eapply trace_range in H11; eauto.
+           simpl in H11.
+           omega.
+           inv H1.
+      * apply in_app_iff in H0; destruct H0.
+        eapply trace_range in H10; eauto.
+        eapply trace_range in H11; eauto.
+        omega.
+        inv H0.
+        eapply trace_range in H10; eauto.
+        simpl in H10.
+        apply well_formed_range in H6; auto.
+        omega.
+        inv H1.
+  - destruct r as [i j]; simpl in *; subst; simpl.
+    apply NoDup_cons.
+    + intro.
+      rewrite in_app_iff in H; destruct H.
+      * eapply shuffle_in in H; eauto.
+        destruct H.
+        -- eapply trace_range in H10; eauto.
+           simpl in H10.
+           omega.
+        -- eapply trace_range in H11; eauto.
+           simpl in H11.
+           apply well_formed_range in H5; auto.
+           omega.
+      * inv H.
+        discriminate H0.
+        inv H0.
+    + apply nodup_append; unfold disjoint_lists; auto; intros.
+      * apply shuffle_nodup_append in H12;
+          unfold disjoint_lists; auto; intros.
+        eapply trace_range in H11; eauto.
+        eapply trace_range in H10; eauto.
+        omega.
+      * apply NoDup_cons.
+        intro.
+        inv H.
+        constructor.
+      * inv H0.
+        -- eapply shuffle_in in H; eauto.
+           destruct H.
+           eapply trace_range in H10; eauto.
+           simpl in H10.
+           apply well_formed_range in H6; auto.
+           omega.
+           eapply trace_range in H11; eauto.
+           simpl in H11.
+           omega.
+
+        -- inv H1.
+Qed.
+
+(** * Event Systems and Traces *)
+
+Lemma evsys_tr_in:
+  forall t tr ev0,
+    well_formed t ->
+    trace t tr ->
+    ev_in ev0 (ev_sys t) ->
+    In ev0 tr.
+Proof.
+  intros.
+  induction H0; inv H; simpl in H1;
+    try expand_let_pairs; inv H1; simpl; auto.
+  - left. inv H3; auto.
+  - right. inv H3; auto.
+    + apply IHtrace in H5; auto.
+      rewrite in_app_iff; auto.
+    + inv H2. rewrite in_app_iff.
+      right. simpl. left. auto.
+  - apply IHtrace1 in H4; auto.
+    rewrite in_app_iff; auto.
+  - apply IHtrace2 in H5; auto.
+    rewrite in_app_iff; auto.
+  - left. inv H2; auto.
+  - right. inv H2; auto.
+    + inv H1; auto.
+      * apply IHtrace1 in H2; auto.
+        rewrite in_app_iff; auto.
+      * apply IHtrace2 in H2; auto.
+        rewrite in_app_iff.
+        right; rewrite in_app_iff; auto.
+    + inv H1; auto.
+      repeat (rewrite in_app_iff; right).
+      simpl; left; auto.
+  - left. inv H3; auto.
+  - right. inv H3; auto.
+    + inv H2; auto.
+      * apply IHtrace1 in H3; auto.
+        eapply shuffle_in_left in H0; eauto.
+        rewrite in_app_iff; auto.
+      * apply IHtrace2 in H3; auto.
+        eapply shuffle_in_right in H0; eauto.
+        rewrite in_app_iff; auto.
+    + inv H2.
+      apply in_app_iff; right; simpl; auto.
+Qed.
+
+(** The traces associated with an annotated term are compatible with
+    its event system. *)
+
+Theorem trace_order:
+  forall t tr ev0 ev1,
+    well_formed t ->
+    trace t tr ->
+    prec (ev_sys t) ev0 ev1 ->
+    earlier tr ev0 ev1.
+Proof.
+  intros.
+  induction H0; inv H; simpl in H1;
+    try expand_let_pairs; inv H1; simpl; auto.
+  - inv H10; inv H9.
+    + eapply evsys_tr_in in H2; eauto.
+      apply earlier_cons; auto.
+      apply in_app_iff; auto.
+    + inv H2.
+      apply earlier_cons; auto.
+      apply in_app_iff; auto. right; simpl; auto.
+  - inv H9.
+  - inv H9.
+    + inv H10.
+      eapply evsys_tr_in in H8; eauto.
+      apply earlier_cons_shift; auto.
+      apply earlier_append; auto; simpl; auto.
+    + eapply IHtrace in H8; eauto.
+      apply earlier_cons_shift; auto.
+      apply earlier_left; auto.
+    + inv H8.
+  - eapply evsys_tr_in in H10; eauto.
+    eapply evsys_tr_in in H11; eauto.
+    apply earlier_append; auto.
+  - apply IHtrace1 in H10; auto.
+    apply earlier_left; auto.
+  - apply IHtrace2 in H10; auto.
+    apply earlier_right; auto.
+  - inv H10; inv H11.
+    + inv H1.
+      * eapply evsys_tr_in in H2; eauto.
+        apply earlier_cons; auto.
+        apply in_app_iff; auto.
+      * eapply evsys_tr_in in H2; eauto.
+        apply earlier_cons; auto.
+        apply in_app_iff; right;
+          apply in_app_iff; simpl; auto.
+    + inv H1.
+      apply earlier_cons; auto.
+      repeat (apply in_app_iff; right).
+      simpl; auto.
+  - inv H10.
+  - inv H10.
+    + inv H11. inv H4.
+      * eapply evsys_tr_in in H1; eauto.
+        apply earlier_cons_shift; auto.
+        apply earlier_append; auto.
+        apply in_app_iff; right; simpl; auto.
+      * eapply evsys_tr_in in H1; eauto.
+        apply earlier_cons_shift; auto.
+        apply earlier_right; auto.
+        apply earlier_append; simpl; auto.
+    + inv H4.
+      * eapply evsys_tr_in in H10; eauto.
+        eapply evsys_tr_in in H11; eauto.
+        apply earlier_cons_shift; auto.
+        apply earlier_append; auto.
+        apply in_app_iff; left; auto.
+      * apply IHtrace1 in H10; auto.
+        apply earlier_cons_shift; auto.
+        apply earlier_left; auto.
+      * apply IHtrace2 in H10; auto.
+        apply earlier_cons_shift; auto.
+        apply earlier_right; auto.
+        apply earlier_left; auto.
+    + inv H4.
+  - inv H11. inv H12.
+    + inv H2; eapply evsys_tr_in in H3; eauto.
+      * apply earlier_cons; auto.
+        apply shuffle_in_left with (es1:=tr1)(es2:=tr2) in H3; auto.
+        apply in_app_iff; left; auto.
+      * apply earlier_cons; auto.
+        apply shuffle_in_right with (e:=ev1) in H0; auto.
+        apply in_app_iff; left; auto.
+    + inv H2.
+      apply earlier_cons; auto.
+      apply in_app_iff; right; simpl; auto.
+  - inv H11.
+  - inv H11.
+    + inv H12. inv H5.
+      * eapply evsys_tr_in in H2; eauto.
+        apply shuffle_in_left with (e:= ev0) in H0; auto.
+        apply earlier_cons_shift; auto.
+        apply earlier_append; simpl; auto.
+      * eapply evsys_tr_in in H2; eauto.
+        apply shuffle_in_right with (e:=ev0) in H0; auto.
+        apply earlier_cons_shift; auto.
+        apply earlier_append; simpl; auto.
+    + inv H5.
+      * apply IHtrace1 in H11; auto.
+        apply shuffle_earlier_left
+          with (e0:=ev0)(e1:=ev1) in H0; auto.
+        apply earlier_cons_shift; auto.
+        apply earlier_left; auto.
+      * apply IHtrace2 in H11; auto.
+        apply shuffle_earlier_right
+          with (e0:=ev0)(e1:=ev1) in H0; auto.
+        apply earlier_cons_shift; auto.
+        apply earlier_left; auto.
+    + inv H5.
+Qed.
